Add initialization functions
Note that these are described and specified in any odd way, so we should
document what we did and prove theorems showing the relational style is
equivalent to something more natural.

src/Spec/Layer.v
@@ -12,13 +12,16 @@ Record Layer Op :=
     sem: Dynamics Op State;
     initP: State -> Prop }.
 
+Inductive InitStatus := Initialized | InitFailed.
+
 (* LayerImpl is just the code needed to translate from one layer to another -
    the logical components are in [LayerRefinement] *)
 Record LayerImpl C_Op Op :=
   { compile_op `(op: Op T) : proc C_Op T;
     (* TODO: layer implementations should be allowed to return from recovery
          (though it's unclear what purpose that would serve *)
-    recover: proc C_Op unit; }.
+    recover: proc C_Op unit;
+    init: proc C_Op InitStatus; }.
 
 Fixpoint compile Op C_Op `(impl: LayerImpl C_Op Op) T (p: proc Op T) : proc C_Op T :=
   match p with
@@ -73,7 +76,11 @@ Section Layers.
       compile_op_ok : compile_op_refines_step impl absr;
       recovery_noop_ok : recovery_refines_crash_step impl absr;
       (* TODO: prove implementations are well-formed *)
-      init_ok : test c_initP ---> any (T:=unit);; test a_initP;; absr }.
+      init_ok : test c_initP;; c_exec impl.(init) --->
+                                                  (any (T:=unit);; test a_initP;; absr;; pure Initialized)
+                (* failing initialization can do anything since a lower layer
+                might have initialized before this failure *)
+                + (any (T:=unit);; pure InitFailed)}.
 
   Context (rf: LayerRefinement).
   Notation compile_op := rf.(impl).(compile_op).
@@ -201,27 +208,51 @@ Section Layers.
     split; [ now apply compile_exec_ok | now apply compile_rexec_ok ].
   Qed.
 
+  Definition ifInit (inited:InitStatus) A `(r: relation A A T) :
+    relation A A (option T) :=
+    if inited
+    then v <- r; pure (Some v)
+    else pure None.
+
   Theorem complete_exec_ok : forall T (p: a_proc T),
-      test c_initP;; c_exec (compile p) --->
-           any (T:=unit);; test a_initP;; (v <- a_sem.(exec) p; any (T:=unit);; pure v).
+      test c_initP;; (inited <- c_exec rf.(impl).(init); ifInit inited (c_exec (compile p))) --->
+           (any (T:=unit);; test a_initP;; (v <- a_sem.(exec) p; any (T:=unit);; pure (Some v))) +
+      (any (T:=unit);; pure None).
   Proof.
     intros.
+    rewrite <- bind_assoc.
     rew rf.(init_ok).
-    rew compile_exec_ok.
-    repeat rel_congruence.
-    apply to_any.
+    repeat setoid_rewrite bind_dist_r; norm.
+    simpl.
+    Split.
+    - Left.
+      rel_congruence.
+      rel_congruence.
+      left assoc rew (compile_exec_ok p).
+      repeat rel_congruence.
+      apply to_any.
+    - Right.
   Qed.
 
   Theorem complete_rexec_ok : forall T (p: a_proc T) R (rec: a_proc R),
-      test c_initP;; c_sem.(rexec) (compile p) (compile_rec rec) --->
-                                   any (T:=unit);; test a_initP;; (v <- a_sem.(rexec) p rec; any (T:=unit);; pure v).
+      test c_initP;; (inited <- c_exec rf.(impl).(init); ifInit inited (c_sem.(rexec) (compile p) (compile_rec rec))) --->
+           (any (T:=unit);; test a_initP;; (v <- a_sem.(rexec) p rec; any (T:=unit);; pure (Some v))) +
+      (any (T:=unit);; pure None).
   Proof.
     intros.
+    rewrite <- bind_assoc.
     rew rf.(init_ok).
-    rew compile_rexec_ok.
-    unfold rexec; norm.
-    repeat rel_congruence.
-    apply to_any.
+    repeat setoid_rewrite bind_dist_r; norm.
+    simpl.
+    Split.
+    - Left.
+      rel_congruence.
+      rel_congruence.
+      rewrite <- bind_assoc.
+      rew compile_rexec_ok.
+      repeat rel_congruence.
+      apply to_any.
+    - Right.
   Qed.
 
 End Layers.
@@ -236,11 +267,16 @@ Definition layer_impl_compose
   : LayerImpl Op1 Op3.
 Proof.
   refine {| compile_op T op :=
-                   impl1.(compile) (impl2.(compile_op) op);
-                 recover := Bind impl1.(recover)
-                                       (fun (_:unit) =>
-                                          impl1.(compile) impl2.(recover))
-              |}.
+              impl1.(compile) (impl2.(compile_op) op);
+            recover := Bind impl1.(recover)
+                                    (fun (_:unit) =>
+                                       impl1.(compile) impl2.(recover));
+            init := Bind impl1.(init)
+                                 (fun inited =>
+                                    if inited
+                                    then impl1.(compile) impl2.(init)
+                                    else Ret InitFailed);
+         |}.
 Defined.
 
 Definition layer_compose
@@ -281,9 +317,21 @@ Proof.
     rew H.
     rew rf1.(rexec_star_rec).
     left assoc rew rf2.(crash_step_refinement).
-  - rew rf1.(init_ok).
-    rew rf2.(init_ok).
+  - unfold layer_impl_compose; simpl.
     rewrite <- bind_assoc.
-    rel_congruence.
-    apply to_any.
+    rew rf1.(init_ok).
+    Split.
+    + rew rf1.(compile_exec_ok).
+      setoid_rewrite <- bind_assoc at 2.
+      rew rf2.(init_ok).
+      repeat (setoid_rewrite bind_dist_r ||
+              setoid_rewrite bind_dist_l); norm.
+      left assoc rew any_idem.
+      Split.
+      * Left.
+      * Right.
+        rewrite <- bind_assoc.
+        rel_congruence.
+        apply to_any.
+    + Right.
 Qed.
